## Pascal's Triangle
[[Maths]]
#10/9/24

$(1-2x)^3$
1 x 1^3  -> 1
3 x 1^2 x (-2x) -> $-6x$
3 x 1 x $(-2x)^2$ -> $12x^2$
1 x $(-3x)^3$ -> $-8x^3$

= 1 - 6x + 12x^2 - 8x^3

Getting a single term in the expansion
The coefficient of $x^2$ in the expansion of $(2-cx)^5$ is 720
Find the possible values of he constant c

$(2-cx)^5$ = 
1 x $2^5$
5 x $2^4$ x - cx
10 x $2^3$ x $(-cx)^2$ 
= $80c^2x^2$

$80c^2$ = $220$
$c^2$ = $9$
$c$ = $3$ or $c$ = $-3$

#### Find the first 3 terms of the binomial expansion of $(2+kx)^7$ 
When $k$ is a constant

$(2+kx)^7$ 
$1$ x $2^7$ -> 128
$7$ x $2^6kx$ -> $448kx$
$21$ x $2^5$ $(kx)^2$ -> $672k^2x^2$

= $128$ + $448kx$ + $672k^2x^2$ 

b) $672k^2$ = $6 x 448k$
/6
$112k^2$ = $448k$
$k^2$ = $4k$
$k^2$ - $4k$ = 0
$k(k-4)$ = 0
$k$ = 0     k = 4

---------------------
### Bracket Expansion

1) $(a+b)^0$ = $a^0$ = 1
2) $(a+b)^1$ = $1a+1b$
3) $(a+b)^2$ = $(a+b)(a+b)$ = $a^2$ + $2ab$ + $b^2$
4) $(a+b)^3$ = $(a+b)(a+b)(a+b)$
	= $(a+b)(a^2 = 2ab + b^2)$ 
	    = $a^3$ + $3a^2b$ + $3ab^2$ + $b^3$ 
##### The Powers of a and b:
a decreases throughout, starting at the power of the original equation.
b increases, starting at 0.